\documentclass{article}

\begin{document}

\section{Bernoulli numbers}

Show that the Laurent development of
$$ \frac{1}{e^z - 1} $$
at the origin is of the form
$$ \frac{1}{z} - \frac{1}{2} + \sum_{k=1}^\infty (-1)^{k-1} \frac{B_k}{(2k)!} z^{2k-1}, $$
where the numbers $B_k$ are known as Bernoulli numbers.  Calculate $B_1, B_2, B_3$.

The singular part of $1/(e^z - 1)$ at $z = 0$ is easily computed to be $1/z$, so we consider $1/(e^z - 1) - 1/z$.  Then this function is analytic in a disk around the origin, so we can Taylor expand.

We clever let
$$ f(z) = \frac{1}{e^z - 1} - \frac{1}{z} + \frac{1}{2}. $$
Then compute $f(z) + f(-z)$ to get that
\begin{eqnarray*}
f(z) + f(-z) &=& \frac{1}{e^z - 1} - \frac{1}{z} + \frac{1}{2} + \frac{1}{e^{-z} - 1} - \frac{1}{-z} + \frac{1}{2} \\
&=& 1 + \frac{(e^{-z} - 1) + (e^z - 1)}{(e^z - 1)(e^{-z} - 1)} \\
&=& 1 + \frac{(e^{-z} - 1) + (e^z - 1)}{1 + 1 - e^{-z} - e^{z}} \\
&=& 1 + \frac{e^{-z} + e^z - 2}{2 - e^{-z} - e^{z}} = 0, \\
\end{eqnarray*}
so $f(z) = -f(-z)$.  Since the function is odd, all of the even terms vanish.  Thus, we have
$$ f(z) = \sum_{k=1}^\infty a_{2k-1} z^{2k-1}. $$
Thus, we have that for some numbers $B_k$ where $a_{2k-1} = (-1)^{k-1} B_k/(2k)!$,
$$ \frac{1}{e^z - 1} = \frac{1}{z} - \frac{1}{2} + \sum_{k=1}^\infty \frac{(-1)^{k-1}}{(2k)!} B_k z^{2k-1}. $$

We compute the first few terms of this series just by differentiating,
$$ f(z) = \frac{z}{12} - \frac{z^3}{720} + \frac{z^5}{30240} + [z^7]. $$
Thus, the coefficient on the first term must be,
$$ \frac{1}{12} = \frac{(-1)^{1-1}}{2!} B_1, $$
so $B_1 = 1/6$.  Furthermore,
$$ -\frac{1}{720} = \frac{(-1)^{2-1}}{4!} B_2, $$
so $B_2 = 1/30$.  Finally,
$$ \frac{1}{30240} = \frac{(-1)^{3-1}}{6!} B_3, $$
so $B_3 = 1/42$.

$B_1 = 1/6$, $B_2 = −1/30$, $B_3 = 1/42$, $B_4 = −1/30$, $B_5 = 5/66$,
$B_6 = −691/2730$, $B_7 = 7/6$, \ldots


\section{Tangent and cotangent}

Express the Taylor development of $\tan z$ and the Laurent development of $\cot z$ in terms of the Bernoulli numbers.

We recall that
$$ \sin x = \frac{1}{2i} (e^{ix} - e^{-ix}), \mbox{ and } \cos x = \frac{1}{2} (e^{-ix} + e^{ix}). $$
But $\cot z = \cos z / \sin z$, so
$$ \cot x = i \frac{e^{-ix} + e^{ix}}{e^{ix} - e^{-ix}}. $$
Multiplying the numerator and denominator by $e^{ix}$ to get,
$$ \cot x = i \frac{1 + e^{2ix}}{e^{2ix} - 1}. $$
Expand the numerator to get
$$ \cot x = \frac{i}{e^{2ix} - 1} + \frac{ie^{2ix}}{e^{2ix} - 1}, $$
which simplifies furhter into
$$ \cot x = \frac{i}{e^{2ix} - 1} + \frac{-i}{e^{-2ix} - 1}. $$
Substituting in the answer from the previous problem, now that we have them in the right form, gives
\begin{eqnarray*}
\cot x &=& i\left(\frac{1}{2ix} - \frac{1}{2} + \sum_{k=1}^\infty (-1)^{k-1} \frac{B_k}{(2k)!} (2ix)^{2k-1}\right) - \\ &\null&  i\left(\frac{1}{-2ix} - \frac{1}{2} + \sum_{k=1}^\infty (-1)^{k-1} \frac{B_k}{(2k)!} (-2ix)^{2k-1}\right)
\end{eqnarray*}
We distribute
\begin{eqnarray*}
\cot x &=& \frac{1}{2x} - \frac{i}{2} + i \sum_{k=1}^\infty (-1)^{k-1} \frac{B_k}{(2k)!} (2ix)^{2k-1} + \\ &\null& \frac{1}{2x} + \frac{i}{2} - i \sum_{k=1}^\infty (-1)^{k-1} \frac{B_k}{(2k)!} (-2ix)^{2k-1},
\end{eqnarray*}
and then cancel the terms
$$
\cot x = \frac{1}{x} + i \sum_{k=1}^\infty (-1)^{k-1} \frac{B_k}{(2k)!} (2ix)^{2k-1} - i \sum_{k=1}^\infty (-1)^{k-1} \frac{B_k}{(2k)!} (-2ix)^{2k-1}
$$
Now make the sums look the same:
$$
\cot x = \frac{1}{x} + i \sum_{k=1}^\infty (-1)^{k-1} \frac{B_k}{(2k)!} (2ix)^{2k-1} + i \sum_{k=1}^\infty (-1)^{k-1} \frac{B_k}{(2k)!} (2ix)^{2k-1},
$$
so we can combine them
$$
\cot x = \frac{1}{x} + 2i \sum_{k=1}^\infty (-1)^{k-1} \frac{B_k}{(2k)!} (2ix)^{2k-1}.
$$
Expand further to get
$$
\cot x = \frac{1}{x} + i \sum_{k=1}^\infty 2^{2k} (-1)^{k-1} \frac{B_k}{(2k)!} (ix)^{2k-1},
$$
and observe that $i^{2k-1} = (-1)^{k+1} i$, so
\begin{eqnarray*}
\cot x &=& \frac{1}{x} + i \sum_{k=1}^\infty 2^{2k} (-1)^{k-1} (-1)^{k+1} i \frac{B_k}{(2k)!} x^{2k-1} \\
&=& \frac{1}{x} - \sum_{k=1}^\infty 2^{2k} \frac{B_k}{(2k)!} x^{2k-1},
\end{eqnarray*}
which is the desired expansion.

For tangent, we recall the obscure trigonometric identity, $\cot z - 2 \cot (2z) = \tan z$.  The singular part of the Laurent expansion above vanishes, and we're just left with the Taylor series.  Explicitly,
\begin{eqnarray*}
\tan z &=& \cot z - 2 \cot (2z) \\
&=& \left(\frac{1}{z} - \sum_{k=1}^\infty 2^{2k} \frac{B_k}{(2k)!} z^{2k-1}\right) - 2 \left(\frac{1}{2z} - \sum_{k=1}^\infty 2^{2k} \frac{B_k}{(2k)!} (2z)^{2k-1}\right) \\
&=& - \sum_{k=1}^\infty 2^{2k} \frac{B_k}{(2k)!} z^{2k-1} + 2  \sum_{k=1}^\infty 2^{2k} \frac{B_k}{(2k)!} (2z)^{2k-1} \\
&=& - \sum_{k=1}^\infty 2^{2k} \frac{B_k}{(2k)!} z^{2k-1} + \sum_{k=1}^\infty 2^{4k} \frac{B_k}{(2k)!} z^{2k-1} \\
&=& \sum_{k=1}^\infty (2^{4k} - 2^{2k}) \frac{B_k}{(2k)!} z^{2k-1}
\end{eqnarray*}



\end{document}


